added factorial and leb

arith.v
@@ -18,9 +18,11 @@ Local Notation "e ⦃  x ⇠ v ⦄" := (@set_env _ _ Var_eq_dec e x v).
 
 Section arith.
 
-  Variables (u x y z : Var) (Hxy : x <> y) (Hxz : x <> z) (Hyz : y <> z).
+  Variables (u x y z : Var) (Hxy : x <> y) (Hxz : x <> z) (Hyz : y <> z) (Hux : u <> x).
 
-  Variable (p_add p_mul p_size : Fun).
+  Variable (p_add p_mul p_fact p_size 
+            p_leb 
+            : Fun).
 
   Definition fe_add := 
     MATCH £u WITH
@@ -38,6 +40,22 @@ Section arith.
            ø   ⇒ ø
         OR x#y ⇒ CALL p_add ON (£z#CALL p_mul ON (£y#£z)).
 
+  Definition fe_fact :=
+    MATCH £u WITH
+         ø   ⇒ ø#ø 
+      OR x#x ⇒ CALL p_mul ON (£u#CALL p_fact ON £x). 
+
+  Definition fe_leb :=
+    MATCH £u WITH
+         ø   ⇒ ø 
+      OR u#x ⇒ 
+      MATCH £u WITH
+           ø   ⇒ ø#ø 
+        OR u#u ⇒ 
+        MATCH £x WITH
+           ø   ⇒ ø 
+        OR x#x ⇒ CALL p_leb ON (£u#£x).
+
   Definition fe_size :=
     MATCH £u WITH
          ø   ⇒ ø#ø
@@ -48,10 +66,14 @@ Section arith.
            
            (Hparam_add : param p_add = u)    
            (Hparam_mul : param p_mul = u)
+           (Hparam_fact : param p_fact = u)
+           (Hparam_leb : param p_leb = u)
            (Hparam_size : param p_size = u) 
 
            (Hbody_add : body p_add = fe_add) 
            (Hbody_mul : body p_mul = fe_mul)
+           (Hbody_fact : body p_fact = fe_fact)
+           (Hbody_leb : body p_leb = fe_leb)
            (Hbody_size : body p_size = fe_size).
 
   Notation "f // s ~~> v" := (fun_sem param body f s v).
@@ -91,6 +113,44 @@ Section arith.
       1: apply fs_var; rew env.
       apply IH2.
       constructor 3; apply fs_var; rew env.
+  Qed.
+
+  Fact fe_fact_spec f e a : f // e ~~> a -> CALL p_fact ON f // e ~~> bt_fact a.
+  Proof.
+    revert f e; induction a as [ | v _ a IHa ]; intros f e H;
+      constructor 7 with (1 := H); rewrite Hbody_fact, Hparam_fact; unfold fe_fact.
+    + constructor 4.
+      1: apply fs_var; rew env.
+      constructor 3; constructor 2.
+    + constructor 5 with v a.
+      1: apply fs_var; rew env.
+      apply fe_mul_spec; fold bt_fact.
+      constructor 3.
+      * apply fs_var; rew env.
+      * apply IHa, fs_var; rew env.
+  Qed.
+
+  Fact fe_leb_spec f e a b : f // e ~~> ⟨a,b⟩ -> CALL p_leb ON f // e ~~> bt_nat_le a b.
+  Proof.
+    revert f e b; induction a as [ | p _ a IHa ]; intros f e b H; 
+      constructor 7 with (1 := H); rewrite Hbody_leb, Hparam_leb; unfold fe_leb.
+    + constructor 5 with ω b.
+      1: apply fs_var; rew env.
+      constructor 4.
+      1: apply fs_var; rew env.
+      constructor 3; constructor 2.
+    + constructor 5 with ⟨p,a⟩ b.
+      1: apply fs_var; rew env.
+      constructor 5 with p a.
+      1: apply fs_var; rew env.
+      destruct b as [ | q b ].
+      * constructor 4.
+        1: apply fs_var; rew env.
+        constructor 2.
+      * constructor 5 with q b.
+        1: apply fs_var; rew env.
+        apply IHa.
+        constructor 3; apply fs_var; rew env.
   Qed.
 
   Fact fe_size_spec f e t : f // e ~~> t -> CALL p_size ON f // e ~~> bt_size t.
